** Preliminaries
*** General state
\begin{equation*}
\left(
    \begin{matrix}
    a \\
    b
    \end{matrix}
\right)
 = a\left|\uparrow\right \rangle+ b\left|\downarrow\right \rangle
\end{equation*}

$|a|^2 + |b|^2 = 1$

*** Pauli Matrices
\begin{equation*}
\hat{\sigma}_x= \left(
    \begin{matrix}
        0 & 1 \\
        1 & 0
    \end{matrix}
\right)
\end{equation*}
\begin{equation*}
\hat{\sigma}_y= \left(
    \begin{matrix}
        0 & -i \\
        i & 0
    \end{matrix}
\right)
\end{equation*}
\begin{equation*}
\hat{\sigma}_z= \left(
    \begin{matrix}
        1 & 0 \\
        0 & -1
    \end{matrix}
\right)
\end{equation*}
\begin{equation*}
\sigma_0 = \left(
    \begin{matrix}
        1 & 0 \\
        0 & 1
    \end{matrix}
\right)
\end{equation*}

*** Bloch Vector

With
$\vec{\sigma} = \hat{\sigma}_x\hat{x} + \hat{\sigma}_y\hat{y} + \hat{\sigma}_z\hat{z}$

\begin{equation*}
\vec{n} = \left\langle \vec{\sigma} \right\rangle = \left\langle \hat{\sigma}_x \right\rangle \hat{x} + \left\langle \hat{\sigma}_y \right\rangle \hat{y}+ \left\langle \hat{\sigma}_z \right\rangle \hat{z}
\end{equation*}

*** Bloch sphere

#+begin_src python
 from qutip import * import matplotlib.pyplot as plt
 fig, ax = plt.subplots(figsize=(0.5,0.5))
 b = Bloch()
 b.axesinstance = ax
 b.zlabel = [r'$|\uparrow\rangle$', r'$|\downarrow\rangle$']
 b.make_sphere()
 plt.show()
#+end_src

* Unitary Evolution with Pure States
** General Unitary Hamiltonian
If we constrain ourselves to unitary evolution, we can parameterize the
general Hamiltonian for a two-level system in terms of a Bloch vector
$\vec{r}$
\begin{equation*}
\vec{r} = r\cos\phi\sin\theta\hat{x} + r\sin\phi\sin\theta\hat{y} + r\cos\theta\hat{z}
\end{equation*}

So that the general Hamiltonian is:
\begin{equation*}
H = \sigma_0r_0+ \vec{\sigma}\cdot\vec{r}
\end{equation*}
\begin{equation*}
H = \left(
    \begin{matrix}
        r_0 + r\cos\theta & re^{-i\phi}\sin\theta \\
        re^{i\phi}\sin\theta & r_0 - r\cos\theta
    \end{matrix}
\right)
\end{equation*}

*** Eigenvalues
\begin{equation*}
\lambda_{1,2} = r_0 \pm r
\end{equation*}

*** Eigenvectors
\begin{equation*}
|\lambda_1\rangle = 
\left(\begin{matrix}
    \cos\frac{\theta}{2}\\
    e^{i\phi}\sin\frac{\theta}{2}
\end{matrix}\right)
= \cos\frac{\theta}{2}\left|\uparrow\right \rangle+ e^{i\phi}\sin\frac{\theta}{2}\left|\downarrow\right \rangle
\end{equation*}
\begin{equation*}
|\lambda_2\rangle =
\left(\begin{matrix}
    e^{i\phi}\sin\frac{\theta}{2}\\
    -\cos\frac{\theta}{2}
\end{matrix}\right)
= e^{i\phi}\sin\frac{\theta}{2}\left|\uparrow\right \rangle-\cos\frac{\theta}{2}\left|\downarrow\right \rangle
\end{equation*}

*** Eigenbasis
\begin{equation*}
\Lambda = 
\left(
    \begin{matrix}
    |\lambda_1\rangle & |\lambda_2\rangle
    \end{matrix}
\right)
=
\left(
    \begin{matrix}
    \left\langle \uparrow \right|\lambda_1 \rangle & \left\langle \uparrow \right|\lambda_2\rangle \\
    \left\langle \downarrow \right|\lambda_1 \rangle & \left\langle \downarrow \right|\lambda_2\rangle
    \end{matrix}
\right)
=
\left(
    \begin{matrix}
    \cos\frac{\theta}{2} & e^{i\phi}\sin\frac{\theta}{2} \\
    e^{i\phi}\sin\frac{\theta}{2} & -\cos\frac{\theta}{2}
    \end{matrix}
\right)
\end{equation*}
\begin{equation*}
\Lambda^{\dagger} = \left(
    \begin{matrix}
    \langle \lambda_1 \left|\uparrow\right \rangle& \langle \lambda_1\left|\downarrow\right \rangle\\
    \langle \lambda_2 \left|\uparrow\right \rangle& \langle \lambda_2\left|\downarrow\right \rangle
    \end{matrix}
\right)
=
\left(
    \begin{matrix}
    \cos\frac{\theta}{2} & e^{-i\phi}\sin\frac{\theta}{2} \\
    e^{-i\phi}\sin\frac{\theta}{2} & -\cos\frac{\theta}{2}
    \end{matrix}
\right)
\end{equation*}

\begin{equation*}
\det(\Lambda) = -e^{i\phi}\left(e^{-i\phi}\cos^2\frac{\theta}{2} + e^{i\phi}\sin^2\frac{\theta}{2}\right)
\end{equation*}

*** Time Evolution

$U(t) = e^{-iHt}$

$U^\dagger(t) U(t) =1$

\begin{equation*}
|\psi (t)\rangle = e^{-iHt}|\psi(0)\rangle = \sum_{k=1}^2 e^{-i\lambda_k t}|\lambda_k\rangle\langle \lambda_k | \psi(0)\rangle =  \sum_{k=1}^2 c_k e^{-i\lambda_k t}|\lambda_k\rangle
\end{equation*}

\begin{equation*}
c_k = \langle\lambda_k|\psi(0)\rangle
\end{equation*}

**** Matrix Elements
\begin{equation*}
\langle j |e^{-iHt} | k \rangle
=
\sum_{\ell}^2 e^{-i\lambda_\ell t}\langle j|\lambda_\ell\rangle\langle \lambda_\ell | k\rangle
\end{equation*}

\begin{equation*}
U = \Lambda
\left(\end{matrix}
e^{-i\lambda_1 t}
&
0
\\
0
&
e^{-i\lambda_2 t}
\end{matrix}\right)
\Lambda^{\dagger}
\end{equation*}

\begin{equation*}
U_{jk}(t) = \sum_{\ell}e^{i\lambda_\ell t}\Lambda_{j\ell}\Lambda^{\dagger}_{\ell k}
\end{equation*}

\begin{equation*}
U = 
\left[
    \end{matrix}
    \cos^2\frac{\theta}{2}e^{-i\lambda_1 t} + \sin^2\frac{\theta}{2}e^{-i\lambda_2 t}
    &
    \frac{1}{2}\sin\theta(e^{-i\phi} e^{-i\lambda_1 t} - e^{i\phi} e^{-i\lambda_2 t})
    \\
    \frac{1}{2}\sin\theta(e^{i\phi} e^{-i\lambda_1 t} - e^{-i\phi} e^{-i\lambda_2 t})
    &
    \sin^2\frac{\theta}{2}e^{-i\lambda_1 t} + \cos^2\frac{\theta}{2}e^{-i\lambda_2 t}
    \end{matrix}
\right]
\end{equation*}

**** Transition Matrix
\begin{equation*}
P_{i\to f}(t) = |U_{jk}|^2(t)
\end{equation*}

** General State Evolution

Starting with the initial state:
\begin{equation*}
|\psi(0)\rangle = |\theta_0,\phi_0\rangle = \cos\frac{\theta_0}{2}\left|\uparrow\right \rangle+ e^{i\phi_0}\sin\frac{\theta_0}{2}\left|\downarrow\right \rangle
\end{equation*}

The evolution of the state under the application of the general
Hamiltonian $H = \vec{\sigma}\cdot\vec{r}$ will become:
\begin{equation*}
|\psi(t)\rangle = a(t)\left|\uparrow\right \rangle+ b(t)\left|\downarrow\right \rangle
\end{equation*}

The explicit expression is given by:
\begin{equation*}
a(t)
= 
i\sin(rt)\sin(\theta)\sin\frac{\theta_0}{2}e^{i(\phi_0 - \phi)} 
+ \left[\cos(rt) - i\sin(rt)\cos(\theta)\right]\cos\frac{\theta_0}{2} 
\end{equation*}

\begin{equation*}
b(t)
= 
e^{i\phi_0}\left[i\sin(rt)\sin(\theta)\cos\frac{\theta_0}{2}e^{-i(\phi_0 - \phi)} + \left[\cos(rt) + i\sin(rt)\cos\theta\right]\sin\frac{\theta_0}{2}\right]
\end{equation*}

We can rewrite this to make the coefficients more amenable to the Bloch
sphere interpretation:
\begin{equation*}
|\psi(t)\rangle = |\Theta(t), \Phi(t)\rangle = \cos\frac{\Theta(t)}{2}\left|\uparrow\right \rangle+ e^{i\Phi(t)}\sin\frac{\Theta(t)}{2}\left|\downarrow\right \rangle
\end{equation*}

where $\Theta(t) = \Theta(\theta, \phi; \theta_0, \phi_0; t)$ and
$\Phi(t) = \Phi(\theta,\phi;\theta_0,\phi_0; t)$ are functions of the:

- $\theta$: polar angle of $\vec{r}$
- $\phi$: azimuthal angle of $\vec{r}$
- $\theta_0$: initial state polar angle
- $\phi_0$: initial state azimuthal angle


** General Bloch Vector Evolution
Starting with the initial Bloch vector:
\begin{equation*}
\vec{n}_0 = \langle \sigma_x(0) \rangle \hat{x} + \langle \sigma_y(0) \rangle \hat{y}+ \langle \sigma_z(0) \rangle \hat{z}
\\
=\cos\phi_0\sin\theta_0\hat{x} + \sin\phi_0\sin\theta_0\hat{y} + \cos\theta_0\hat{z}
\end{equation*}

The Bloch vector will evolve under the General Hamiltonian to:
\begin{equation*}
\vec{n}(t) = \langle \sigma_x(t) \rangle \hat{x} + \langle \sigma_y(t) \rangle \hat{y}+ \langle \sigma_z(t) \rangle \hat{z}
\\
=\cos\Phi(t)\sin\Theta(t)\hat{x} + \sin\Phi(t)\sin\Theta(t)\hat{y} + \cos\Theta(t)\hat{z}
\end{equation*}
