
#+TITLE: Mechanics: From Newton to Schrodinger
#+AUTHOR: Trent Fridey
#+DATE: 2021-10-25
#+HUGO_TAGS: physics math
#+STARTUP: latexpreview
#+HUGO_BASE_DIR: ~/trent/blog
#+HUGO_SECTION: posts/newton-to-schrodinger

* Outline
Newton
  $$
  \sum_i \vec{F}_i = m\vec{a}
  $$

  D'Alembert
  $$
   \sum_i \vec{F}_i - m\vec{a} = 0
  $$
Virtual work
  $$
  \delta W = \sum_i \left(\vec{F}_i - m\vec{a}\right) \cdot \delta \vec{r} = 0
  $$
Generalized coordinates
$$
\vec{r} = \vec{r}(q_1, q_2, \dots, q_n; t)
$$

$$
\vec{v} = \frac{d \vec{r}}{dt} = \frac{\partial \vec{r}}{\partial q_k} \frac{\partial q_k}{\partial t}
$$

$$
\delta \vec{r} = \sum_k \frac{\partial \vec{r}}{\partial q_k} \delta q_k
$$
$$
\delta W = \sum_k \sum_i \left( \vec{F}_i - m \vec{a} \right) \cdot \frac{\partial \vec{r}}{\partial q_k} \delta q_k = 0
$$
$$
Q_k =  \vec{F}_i \cdot \frac{\partial \vec{r}}{\partial q_k}
$$

$$
\frac{\partial \vec{r}}{\partial q_k} = \frac{\partial \vec{r}/\partial t}{\partial q_k /\partial t} = \frac{\partial \vec{v}}{\partial \dot{q}_k}
$$

$$
\vec{a} \cdot \frac{\partial \vec{r}}{\partial q_k} =  \frac{d}{dt}\left(\vec{v}\cdot \frac{\partial \vec{v}}{\partial \dot{q}_k} \right) - \vec{v}\cdot\frac{\partial \vec{v}}{\partial q_k}
$$

$$
\vec{v}\cdot \frac{\partial \vec{v}}{\partial \dot{q}_k} = \frac{1}{2}\frac{\partial}{\partial \dot{q}_k}(\vec{v}\cdot\vec{v})
$$

$$
\vec{v}\cdot\frac{\partial \vec{v}}{\partial q_k} = \frac{1}{2}\frac{\partial}{\partial q_k}(\vec{v}\cdot \vec{v})
$$

$$
\vec{a}\cdot\frac{\partial \vec{r}}{\partial q_k}
=
\frac{1}{2}\left(\frac{d}{dt}\frac{\partial}{\partial \dot{q}_k} - \frac{\partial}{\partial q_k} \right)(\vec{v}\cdot\vec{v})
$$

$$
\delta W = \sum_{k} \left[ Q_k -\frac{1}{2}m\left(\frac{d}{dt}\frac{\partial}{\partial \dot{q}_k} - \frac{\partial}{\partial q_k} \right)(\vec{v}\cdot\vec{v})\right]  \delta q_k
$$

$$
T = \frac{1}{2}m(\vec{v}\cdot\vec{v})
$$

$$
\delta W = \sum_k \left[ Q_k - \left(\frac{d}{dt}\frac{\partial T}{\partial \dot{q}_k} - \frac{\partial T}{\partial q_k} \right) \right]\delta q_k
$$

$$
Q_k = \frac{\partial V}{\partial q_k}
$$

$$
\frac{\partial V}{\partial \dot{q}_k} = 0
$$

$$
L = T - V
$$

$$
\delta W = \sum_k \left[
\left(\frac{d}{dt}\frac{\partial L}{\partial \dot{q}_k} - \frac{\partial L}{\partial q_k} \right)\right] \delta q_k
\right]
$$
Lagrange
$$
\left(\frac{d}{dt}\frac{\partial L}{\partial \dot{q}_k} - \frac{\partial L}{\partial q_k} \right) = 0
$$

$$
dL = \frac{\partial L}{\partial \dot{q}}d\dot{q} + \frac{\partial L}{\partial q}dq
$$
Hamilton
$$
dH = d(L - p\dot{q}) = (\frac{\partial L}{\partial \dot{q}} - p)d\dot{q} + \frac{\partial L}{\partial q}dq - \dot{q}dp
$$

$$
\frac{\partial L}{\partial \dot{q}} - p = 0
$$

$$
dH = \frac{\partial H}{\partial q}dq + \frac{\partial H}{\partial p}dp
$$

$$
\frac{\partial H}{\partial p} = -\dot{q}  
$$

$$
\frac{\partial H}{\partial q} = \frac{\partial L}{\partial q} = -\frac{d}{dt}\frac{\partial L}{\partial \dot{q}} = \dot{p}
$$

Canonical transformations

$$
L' = L + \frac{dG(q,t)}{dt}
$$

$$
\frac{dG}{dt} = \frac{\partial G}{\partial q}\frac{d q}{d t} + \frac{\partial G}{\partial t}
$$

$$
\frac{d}{dt}\frac{\partial }
\frac{d}{dt}\frac{\partial }{\partial \dot{q}}(L + \frac{dG(q,t)}{dt}) =
\frac{\partial}{\partial q}(L + \frac{dG(q,t)}{dt})
$$

$$
\frac{d}{dt}\frac{\partial L}{\partial \dot{q}} - \frac{\partial L}{\partial q}
$$







 HJE

 Choose $Q, P$ such that $H(Q, P, t) = 0 \implies \dot{Q} = \dot{P} = 0$, restricted to canonical transformations. Make a /generating function/ $S(q,Q,t)$ to do effect this, solve for it instead of solving differential equations.


 $$
 H\left(q, \frac{\partial S}{\partial q}, t \right) + \frac{\partial S}{\partial t} = 0
 $$

 Schrodinger

 $$
 S = k\log(\psi)
 $$

 $$
 H\left(q, \frac{k}{\psi}\frac{\partial \psi}{\partial q}, t\right) = E
 $$

 $$
 \frac{1}{2m}\left(\frac{\partial S}{\partial q}\right)^2 + V(q) = E
 $$

 $$
 \frac{k^2}{2m}\left(\frac{\partial \psi}{\partial q}\right)^2 + V(q)\psi^2 = E\psi^2
 $$

 $$
 J = \int \left[
 \frac{k^2}{2m}\left(\frac{\partial \psi}{\partial q}\right)^2 + V(q)\psi^2 - E\psi^2 \right] dq
 $$

 $$
 \delta J = 0 
 $$

 $$
 \delta J = \int \left[\frac{k^2}{2m}\delta \left(\frac{\partial \psi}{\partial q}\right)^2 + 2(V(q) - E)\psi \delta \psi \right] dq
 $$

 $$
 \int \delta\left(\frac{\partial \psi}{\partial q}\right)^2 dq = \left. \frac{\partial \psi}{\partial q}\delta\psi\right|_{\partial \Omega} - \int \frac{\partial^2 \psi}{\partial q^2} \delta\psi dq
 $$

 $$
 \frac12 \delta J = \int \left[-\frac{k^2}{2m}\frac{\partial^2 \psi}{\partial q^2} + (V(q) - E)\psi \right]\delta \psi dq = 0
 $$

 $$
-\frac{k^2}{2m}\frac{\partial^2 \psi}{\partial q^2} + V(q)\psi = E\psi
 $$

 QED
